The power rule is a method used to find the derivative of functions that are in the form f of x equals x raised to the power of n. The formula for this rule is:

$$\frac{d}{dx}(x^n) = nx^{n-1}$$

For example, if we have the function f of x equals x cubed, its derivative would be:

$$\frac{d}{dx}(x^3) = 3x^2$$

The chain rule, on the other hand, helps us find the derivative of composite functions. If we have a function g of x inside another function f of x, we can use the chain rule to find its derivative. The formula for this rule is:

$$(f(g(x)))' = f'(g(x)) \cdot g'(x) $$

To better understand how it works, let's consider an example where we have a composite function: 

Suppose we have the function f of x equals (x squared plus 1) raised to the power of 3. We can think of this as a composite function where g(x) equals (x squared plus 1). Using the chain rule, we can find its derivative as follows:

Firstly, let's calculate g'(x), which is equal to:

$$\frac{d}{dx}(x^2+1)=2x$$

Now let's calculate f'(g(x)), which means finding first derivate with respect to $u=x^2+1$, and then substituting $u=g(x)$.

So,

$${f}'(u)=3u^{2}$$$$ {f}'(g(x))=3{(g(x))}^{2}=3{(x^{2}+1)}^{2} $$


Finally using Chain Rule Formula,

$$(f(g(x)))'={f}'(g(x)).g'(x)=3{(x^{2}+1)}^{2}.2x$$

Therefore, the derivative of f of x equals (x squared plus 1) raised to the power of 3 is:

$$(f(x))' = 6x(x^2 + 1)^2 $$

In summary, derivatives are essential in calculus and help us find rates of change or maximum and minimum values of functions. We can use different methods such as the power rule and chain rule to calculate them.